il/Env.v
@@ -6,12 +6,12 @@ Export BMap.
 
 (** ** Type Environments *)
 (** Value environments are functions from var to a value type X. *)
-Definition onv (X:Type) := map (option X).
-Definition ompty X : onv X := @empty _ (@None X).
+Definition onv (X:Type) := map var (option X).
+Definition ompty X : onv X := @empty _ _ (@None X).
 
 (** ** Value Environments *)
 (** Type environments are functions from var to option X for some type type X *)
-Definition env (X:Type) `{Defaulted X} := map X.
+Definition env (X:Type) `{Defaulted X} := map var X.
 Definition empty (V:Type) `{Defaulted V} : env V := empty default_el.
 
 (* 
